Protocol.thy: add embedding

Protocol.thy
@@ -7,19 +7,49 @@ type_synonym var = string
 type_synonym const = string
 datatype msg =
 Hash msg | Concat msg msg | Sym_encrypt msg msg | Pub_encrypt msg msg | Sign msg msg
-| Const const | Var var
+| Const const | Variable var
 (* Pub_encrypt content key  and so on*)
 
+(* embedding *)
 datatype symbol =
-SHash | SConcat | SSym_encrypt | SPub_encrypt | SSign | SConst | SVar
+SHash | SConcat | SSym_encrypt | SPub_encrypt | SSign | SConst const
 fun arity :: "symbol \<Rightarrow> nat" where
 "arity SHash = 1"
 | "arity SConcat = 2"
 | "arity SSym_encrypt = 2"
 | "arity SPub_encrypt = 2"
 | "arity SSign = 2"
-| "arity SConst = 0"
-| "arity SVar = 0"
+| "arity (SConst _) = 0"
 
+type_synonym msg_term = "(symbol, var) term"
+
+fun embed :: "msg \<Rightarrow> msg_term" where
+"embed (Hash x) = Fun SHash [embed x]"
+| "embed (Concat x y) = Fun SConcat [embed x, embed y]"
+| "embed (Sym_encrypt x y) = Fun SSym_encrypt [embed x, embed y]"
+| "embed (Pub_encrypt x y) = Fun SPub_encrypt [embed x, embed y]"
+| "embed (Sign x y) = Fun SSign [embed x, embed y]"
+| "embed (Const x) = Fun (SConst x) []"
+| "embed (Variable x) = Var x"
+
+fun msg_of_term :: "msg_term \<Rightarrow> msg" where
+"msg_of_term (Fun SHash [x]) = Hash (msg_of_term x)"
+| "msg_of_term (Fun SConcat [x, y]) = Concat (msg_of_term x) (msg_of_term y)"
+| "msg_of_term (Fun SSym_encrypt [x, y]) = Sym_encrypt (msg_of_term x) (msg_of_term y)"
+| "msg_of_term (Fun SPub_encrypt [x, y]) = Pub_encrypt (msg_of_term x) (msg_of_term y)"
+| "msg_of_term (Fun SSign [x, y]) = Sign (msg_of_term x) (msg_of_term y)"
+| "msg_of_term (Fun (SConst x) []) = Const x"
+| "msg_of_term (Var x) = Variable x"
+
+(* embedding lemmas *)
+lemma wf_term_embed [simp]: "wf_term arity (embed msg)"
+  sorry
+
+lemma msg_of_term_embed [simp]: "msg_of_term (embed x) = x"
+proof(induction x)
+qed auto
+
+lemma embed_msg_of_term [simp]: "wf_term arity x \<Longrightarrow> embed (msg_of_term x) = x"
+  sorry
 
 end
